Version of br93 that came out of US school.

examples/br93.ec
@@ -1,351 +1,388 @@
-require import Array.
-require import FMap.
-require import FSet.
-require import Int.
-require import Distr.
-require import Bool.
-require import Real.
-require (*--*) AWord.
-require (*--*) ROM.
+require import Fun Bool Int Real Distr List FSet Array FMap.
+require (*--*) AWord ROM.
 
-op k : int. (* size of message *)
-op l : int. (* size of randmness *)
-op n : int. (* size of cipher *)
+(** We consider three lengths of bitstrings **)
+op k : { int | 0 < k } as k_pos. (* size of message *)
+op l : { int | 0 < l } as l_pos. (* size of randomness *)
+op n : { int | 0 < n } as n_pos. (* size of cipher *)
 
 axiom sizes : k + l = n.
 
-op qH : int. (* bound on adversary calls to hash H *)
+clone import AWord as Plaintext with
+  op length = k
+proof leq0_length by smt.
 
-clone AWord as Plaintext with op length = k.
-clone AWord as Ciphertext with op length = n.
-clone AWord as Randomness with op length = l.
+clone import AWord as Ciphertext with
+  op length = n
+proof leq0_length by smt.
+
+clone import AWord as Randomness with
+  op length = l
+proof leq0_length by smt.
 
 type plaintext = Plaintext.word.
 type ciphertext = Ciphertext.word.
 type randomness = Randomness.word.
 
-import Plaintext.
-import Ciphertext.
-import Randomness.
+(* We only need distributions on plaintexts and nonces *)
+op uniform      = Plaintext.Dword.dword.
+op uniform_rand = Randomness.Dword.dword.
 
-type pkey.
-type skey.
-op keypairs: (pkey * skey) distr.
-op f : pkey -> randomness -> randomness.
-op finv : skey -> randomness -> randomness.
+(* We have operators that combine them *)
+op (||) (x:randomness) (y:plaintext):ciphertext =
+ Ciphertext.from_bits ((to_bits x) || (to_bits y)).
 
-axiom finvof : forall(pk : pkey, sk : skey, x : randomness),
- in_supp (pk,sk) keypairs => finv sk (f pk x) = x.
+(** Please ignore **)
+lemma find_unique x' (p: 'a -> bool) (xs : 'a list):
+  (forall (x : 'a), p x => x = x') =>
+  mem x' xs => p x' => find p xs = Some x'.
+proof.
+  move=> p_unique x'_in_m p_x'.
+  case {-1}(find p xs) (Logic.eq_refl (find p xs))=> //=.
+    smt.
+    by move=> x /List.find_cor [] _ /p_unique.
+qed.
 
-axiom fofinv : forall(pk : pkey, sk : skey, x : randomness),
- in_supp (pk,sk) keypairs => f pk (finv sk x) = x.
+(*** One way trapdoor permutation (pre-instantiated) ***)
+(**  [See theory OW.ec] **)
+theory OWTP.
+  type pkey, skey.
 
-axiom keypair_lossless : mu keypairs predT = 1%r.
+  op keypairs: (pkey * skey) distr.
+  axiom keypair_lossless : is_lossless keypairs.
 
-op uniform : plaintext distr = Plaintext.Dword.dword.
-op uniform_rand : randomness distr = Randomness.Dword.dword.
+  op f       : pkey -> randomness -> randomness.
+  op finv    : skey -> randomness -> randomness.
 
-clone import ROM.SetLog as RandOrcl_BR with 
+  axiom finvof pk sk x:
+   support keypairs (pk,sk) =>
+   finv sk (f pk x) = x.
+
+  axiom fofinv pk sk x:
+   support keypairs (pk,sk) =>
+   f pk (finv sk x) = x.
+
+  lemma f_injective sk pk x y:
+    support keypairs (pk,sk) =>
+    f pk x = f pk y =>
+    x = y.
+  proof.
+    move=> Hsupp Heqf.
+    by rewrite -(finvof pk sk) // Heqf finvof.
+  qed.
+
+  module type Inverter = {
+    proc i(pk:pkey,y:randomness): randomness
+  }.
+
+  module OW(I:Inverter) = {
+    var r:randomness
+
+    proc main(): bool = {
+      var x', pk, sk;
+
+      (pk,sk) = $keypairs;
+      r       = $uniform_rand;
+      x'      = I.i(pk,f pk r);
+      return (r = x');
+    }
+  }.
+
+  (** f is a secure OWTP if, for any inverter I,
+        Adv^{OW}^f(I) = Pr[OW(I).main() @ &m: res]
+      is small. **)
+end OWTP.
+import OWTP.
+
+(*** We make use of a hash function (ROM) from randomness to
+     plaintext. We let the adversary query it qH times at most. ***)
+op qH : { int | 0 < qH } as qH_pos.
+
+clone import ROM.ListLog as RandOrcl_BR with 
   type from  <- randomness, 
   type to    <- plaintext,
-  op dsample <- fun (x:randomness), uniform,
+  op dsample <- fun (x:randomness) => uniform,
   op qH      <- qH.
 import Lazy.
 import Types.
 
+(*** We can now define what it means to be a CPA-secure public-key encryption scheme ***)
+(**  [See theory PKE.ec] **)
 module type Scheme(RO : Oracle) = {
- proc kg() : (pkey * skey)
- proc enc(pk:pkey, m:plaintext): ciphertext 
+  proc kg(): (pkey * skey)
+  proc enc(pk:pkey, m:plaintext): ciphertext 
 }.
 
-module type Adv(ARO : ARO)  = {
- proc a1 (p : pkey) : (plaintext * plaintext) {ARO.o} 
- proc a2 (c : ciphertext) : bool {ARO.o}
+module type Adv(ARO: ARO)  = {
+  proc a1(p:pkey)      : (plaintext * plaintext)
+  proc a2(c:ciphertext): bool
 }.
 
+module CPA(S:Scheme, A:Adv) = {
+  module ARO = Log(RO)
+  module A = A(ARO)
+  module SO = S(RO)
 
-module CPA(S : Scheme, A_ : Adv) = {
- module ARO = Log(RO)
- module A = A_(ARO)
- module SO = S(RO)
   proc main(): bool = {
-  var pk:pkey;
-  var sk:skey;
-  var m0, m1 : plaintext;
-  var c : ciphertext;
-  var b,b' : bool;
-  ARO.init();
-  (pk,sk)  = SO.kg();
-  (m0,m1)  = A.a1(pk);
-  b = ${0,1}; 
-  c  = SO.enc(pk,b?m0:m1);
-  b' = A.a2(c);
-  return b = b';
- } 
+    var pk, sk, m0, m1, c, b, b';
+
+    ARO.init();
+    (pk,sk)  = SO.kg();
+    (m0,m1)  = A.a1(pk);
+    b = ${0,1}; 
+    c  = SO.enc(pk,b?m0:m1);
+    b' = A.a2(c);
+    return b' = b;
+  } 
 }.
 
-op (||) (x:randomness) (y:plaintext):ciphertext =
- Ciphertext.from_bits ((to_bits x) || (to_bits y)).
+(** A Scheme E is IND-CPA secure if, for any A,
+      Adv^{CPA}_{S}(A) = `|Pr[CPA(S,A).main() @ &m: res] - 1/2|
+    is small. **)
 
+module BR(R:Oracle): Scheme(R) = {
+  proc kg():(pkey * skey) = {
+    var pk, sk;
 
-module M = {
- var r : randomness
-}.
-
-module BR(R : Oracle) : Scheme(R) = {
- proc kg():(pkey * skey) = {
-  var (pk, sk): pkey * skey;
-  (pk,sk) = $keypairs;
-  return (pk,sk);
- }
+    (pk,sk) = $keypairs;
+    return (pk,sk);
+  }
  
- proc enc(pk:pkey, m:plaintext): ciphertext = {
-  var h : plaintext;
-  M.r = $uniform_rand; 
-  h  = R.o(M.r);
-  return ((f pk M.r) ||   m ^ h);
- }
+  proc enc(pk:pkey, m:plaintext): ciphertext = {
+    var h, r;
+
+    r = $uniform_rand; 
+    h = R.o(r);
+    return ((f pk r) ||   m ^ h);
+  }
 }.
 
+(** Given a CPA adversary A, we construct a OW inverter **)
+module BR_OW(A:Adv): Inverter = {
+  module ARO = Log(RO)
+  module A = A(ARO)
 
-  (* Step 1: replace the hash call by a random value *)
+  var x:randomness
 
-module BR2(R : Oracle) : Scheme(R) = {
- proc kg():(pkey * skey) = {
-  var (pk, sk): (pkey * skey);
-  (pk,sk) = $keypairs;
-  return (pk,sk);
- }
- 
- proc enc(pk:pkey, m:plaintext): ciphertext = {
-  var h : plaintext;
-  M.r = $uniform_rand; 
-  h = $uniform; 
-  return ((f pk M.r) || h);
- }
+  proc i(pk:pkey,y:randomness): randomness = {
+    var m0,m1,h,b;
+
+    ARO.init();
+    (m0,m1) = A.a1(pk);
+    h = $uniform; 
+    b = A.a2(y || h);
+    x = oget (find (fun p => f pk p = y) ARO.qs);
+    return x;
+  }
 }.
 
-lemma eq1_enc :
- equiv [ BR(RO).enc ~ BR2(RO).enc : 
-={pk,RO.m} ==>
-!mem M.r{2} (dom RO.m{2}) => (={res} /\ eq_except RO.m{1} RO.m{2} M.r{2}) ].
-proof.
- proc;inline RO.o.
- wp;rnd ((^) m{1}) ((^) m{1}).
- wp;rnd;skip;progress => //; try (by algebra); smt.
-qed.
-
-module CPA2(S : Scheme, A_ : Adv) = {
- module ARO = Log(RO)
- module A = A_(ARO)
- module SO = S(RO)
-  proc main(): bool = {
-  var pk:pkey;
-  var sk:skey;
-  var m0, m1 : plaintext;
-  var c : ciphertext;
-  var b,b' : bool;
-  ARO.init();
-  (pk,sk)  = SO.kg();
-  (m0,m1)  = A.a1(pk);
-  c  = SO.enc(pk,m0);
-  b' = A.a2(c);
-  b = ${0,1}; 
-  return b' = b;
- } 
-}.
-
-
-lemma lossless_ARO_init : islossless Log(RO).init.
-proof. by apply (Log_init_ll RO); apply RO_init_ll. qed.
+(** such that Adv^{CPA}_{S}(A) <= Adv^{OW}^{f}(I(A)).
+    We now prove this bound. **)
+lemma lossless_ARO_init: islossless Log(RO).init.
+proof. by apply/(Log_init_ll RO)/RO_init_ll. qed.
 
 lemma lossless_ARO_o : islossless Log(RO).o.
-proof. by apply (Log_o_ll RO); apply RO_o_ll; apply Plaintext.Dword.lossless. qed.
+proof. by apply/(Log_o_ll RO)/RO_o_ll/Plaintext.Dword.lossless. qed.
 
 section.
+  (* Forall CPA adversary A whose memory footprint is disjoint from that of RO, Log and OW *)
+  declare module A : Adv {RO,Log,OW}.
 
-declare module A : Adv {M,RO,Log}.
+  (* and whose two procedures as lossless provided the random oracle is *)
+  axiom a1_ll (O <: ARO{A}): islossless O.o => islossless A(O).a1.
+  axiom a2_ll (O <: ARO{A}): islossless O.o => islossless A(O).a2.
 
-axiom lossless1 : (forall (O <: ARO), islossless O.o =>  islossless A(O).a1).
-axiom lossless2 : (forall (O <: ARO), islossless O.o =>  islossless A(O).a2).
+  (* the following lemmas hold on the following constructions *)
 
-equiv eq1 :  CPA(BR,A).main ~ CPA2(BR2,A).main : 
-(glob A){1} = (glob A){2} ==>
- (!mem M.r Log.qs){2} => ={res}.
-proof.
- proc.
- swap{2} -2.
- call (_ : (mem M.r Log.qs), 
-           (={Log.qs} /\ eq_except RO.m{1} RO.m{2} M.r{2})).
- intros => O Hll;apply (lossless2 O) => //.
- proc;inline RO.o;wp;rnd;wp;skip;progress => //; first 5 last; last 6 smt.
-  case ((x = M.r){2}); first smt.
-  by apply (absurd (mem x (dom RO.m)){2})=> //; smt.
- intros _ _;apply lossless_ARO_o.
- intros &m; proc; wp; call (RO_o_ll _); auto; smt.
- call eq1_enc.
- rnd.
- call  (_: ={RO.m,Log.qs} /\
- (forall (x : randomness), mem x Log.qs{2} <=> mem x (dom RO.m{2}))).
-  proc;inline RO.o;wp;rnd;wp;skip;progress;smt.
-  inline CPA(BR,A).SO.kg CPA2(BR2,A).SO.kg.
-  inline CPA(BR,A).ARO.init CPA2(BR2,A).ARO.init RO.init;wp;rnd;wp;skip.
-  progress;by smt.
-qed.
+  (** Step 1: replace RO call with random sampling **)
+  local module BR1(R:Oracle): Scheme(R) = {
+    var r:randomness
 
-lemma foo1 : forall (b:bool), mu {0,1} (pred1 b) = 1%r / 2%r.
-proof. intros b; apply (Bool.Dbool.mu_x_def b). qed. 
+    proc kg = BR(R).kg
 
-lemma foo2 : mu uniform_rand predT = 1%r.
-proof. apply Randomness.Dword.lossless. qed.
+    proc enc(pk:pkey, m:plaintext): ciphertext = {
+      var h;
 
-lemma foo3 : mu uniform predT = 1%r.
-proof. apply Plaintext.Dword.lossless. qed.
+      r = $uniform_rand;
+      h = $uniform;
+      return ((f pk r) || m ^ h);
+    }
+  }.
 
-lemma prob1_1 : 
- forall &m,Pr[CPA2(BR2,A).main()  @ &m : res] = 1%r / 2%r.
-proof.
- intros &m.
- byphoare (_ : true ==> res); trivial.
-   proc.
-   rnd (pred1 b').
-   conseq ( _ : ==> true).
-    rewrite {2}pred1E; progress; apply foo1.
-   call ( _ :true). 
-   intros => O Hll;apply (lossless2 O) => //.
+  (** The success probability of A in CPA(BR) is bounded by
+      the success probability of A in CPA(BR1) plus the probability
+      of the adversary querying the RO with the randomness used in
+      the challenge encryption. **)
+  local lemma BR_BR1 &m:
+    Pr[CPA(BR,A).main() @ &m: res]
+    <= Pr[CPA(BR1,A).main() @ &m: res]
+       + Pr[CPA(BR1,A).main() @ &m: mem BR1.r Log.qs].
+  proof.
+    byequiv=> //=.
+    proc.
+    (* Until the adversary queries the ROM with r, knowing that
+       the two ROMs agree on all points except r is sufficient
+       to prove the equivalence of the adversary's views        *)
+    call (_: mem BR1.r Log.qs,
+             eq_except RO.m{1} RO.m{2} BR1.r{2}).
+      (* Adversary is lossless *)
+      exact/a2_ll.
+      (* Oracles are equivalent up to the failure event *)
+      proc. inline RO.o.
+      wp. rnd.
+      wp. skip. smt.
+      (* Left oracle is lossless *)
+      move=> &2 _; exact/lossless_ARO_o.
+      (* Right oracle is lossless and preserves bad once set *)
+      move=> &1. proc. inline *. wp. rnd. wp. skip. smt. (* or use conseq... *)
+    (* We return to the main game *)
+    inline CPA(BR,A).SO.enc CPA(BR1,A).SO.enc.
+    inline RO.o.
+    wp. rnd.
+    wp. rnd.
+    wp. rnd.
+    (* The first adversary call is simpler *)
+    call (_:    ={Log.qs, RO.m}
+             /\ (forall x, mem x Log.qs{1} <=> mem x (dom RO.m){1})).
+      proc. inline RO.o.
+      wp. rnd.
+      wp. skip. smt.
+    inline *. auto.
+    progress.
+      smt.
+      smt.
+      smt.
+      smt.
+      smt.
+      smt.
+  qed.
 
-    apply lossless_ARO_o.   
-   inline CPA2(BR2,A).SO.enc;do 2! (wp;rnd predT);wp.
-   conseq ( _ : ==> true).
-     rewrite foo2; rewrite foo3;progress.
-   call (_ : true).
-   intros => O Hll;apply (lossless1 O) => //.
-     apply lossless_ARO_o.  
-   inline CPA2(BR2,A).SO.kg.
-   wp;rnd predT;wp.
-   conseq ( _ : ==> true).
-     progress;apply keypair_lossless. 
-   call lossless_ARO_init;skip;trivial.
-qed.
+  (** Step 2: replace h ^ m with h in challenge encryption **)
+  local module BR2(R:Oracle): Scheme(R) = {
+    var r:randomness
 
-lemma prob1_2 : forall &m,
-Pr[CPA(BR,A).main() @ &m: res] <=
-1%r/2%r + Pr[CPA2(BR2,A).main() @ &m : mem M.r Log.qs].
-proof.
- intros &m.
- rewrite -(prob1_1 &m) //.
- apply (Real.Trans _ 
-             Pr[CPA2(BR2,A).main() @ &m : res \/ mem M.r Log.qs]).
- byequiv (eq1 ) => //;progress;smt.
- rewrite Pr [mu_or].  smt.
-qed.
+    proc kg():(pkey * skey) = {
+      var pk, sk;
 
-module type Inverter = {
- proc i(pk : pkey, y : randomness) : randomness
-}.
+      (pk,sk) = $keypairs;
+      return (pk,sk);
+    }
 
-module OW(I :Inverter) ={
- proc main() : bool ={
- var x : randomness;
- var x' : randomness;
- var y : randomness;
- var pk : pkey;
- var sk : skey;
-  x = $uniform_rand;
-  (pk,sk) = $keypairs;
-  x'  = I.i(pk,(f pk x));
-  return (x = x');
- }
-}.
+    proc enc(pk:pkey, m:plaintext): ciphertext = {
+      var h;
 
-module BR_OW(A_ : Adv) : Inverter = {
- module ARO = Log(RO)
- module A = A_(ARO)
-  proc i(pk : pkey,y : randomness) : randomness ={
-  var m0 : plaintext;
-  var m1 : plaintext;
-  var h : plaintext;
-  var b : bool;
-  var x : randomness;
-  ARO.init();
-  (m0,m1)  = A.a1(pk);
-  h = $uniform; 
-  b  = A.a2(y || h);
-  x = oget (FMap.find (fun p0 p1,f pk p0 = y) RO.m);
-   return (x);
- }
-}.
+      r = $uniform_rand; 
+      h = $uniform; 
+      return ((f pk r) || h);
+    }
+  }.
 
-lemma f_iny x  y pk sk: 
-in_supp (pk,sk) keypairs  =>
-f pk x = f pk y => x = y.
-proof.
- move=> Hsupp Heqf.
- rewrite -(finvof pk sk _ _);first smt.
- rewrite -(finvof pk sk _ _);first smt.
- rewrite Heqf;smt.
-qed.
+  (* The success probabilities in both games are the same *)
+  local lemma BR1_BR2 &m:
+    Pr[CPA(BR1,A).main() @ &m: res]
+    = Pr[CPA(BR2,A).main() @ &m: res].
+  proof.
+    byequiv=> //=.
+    proc.
+    call (_: ={RO.m}).
+      proc. inline *. auto.
+    inline CPA(BR1,A).SO.enc CPA(BR2,A).SO.enc.
+    wp. rnd (fun x => m{2} ^ x).
+    rnd.
+    wp. rnd.
+    call (_: ={RO.m}).
+      proc. inline *. auto.
+    inline *. auto.
+    progress.
+      algebra.
+      smt.
+      smt.
+      algebra.
+  qed.
 
-equiv eq2 : CPA2(BR2,A).main ~ OW(BR_OW(A)).main : 
- (glob A){1} = (glob A){2} ==> (mem M.r{1} Log.qs{1} => res{2}).
-proof.
- proc.
- rnd{1}.
- inline  BR_OW(A).i.
- inline CPA2(BR2, A).ARO.init RO.init CPA2(BR2, A).SO.kg 
- BR_OW(A).ARO.init.
- inline CPA2(BR2,A).SO.enc.
- seq 11 9:
- (={pk,sk,RO.m,Log.qs} /\ pk0{2} = pk{2} /\ 
-  in_supp (pk{2},sk{2}) keypairs /\
-(glob A){1} = (glob A){2}  /\ (forall x, mem x (dom RO.m){1} = mem x Log.qs{1}) /\
- M.r{1} = x{2} /\ y0{2} = f pk{2} x{2}).
+  (* The probability of the failure event is the same in both games *)
+  local lemma BR1_BR2_bad &m:
+    Pr[CPA(BR1,A).main() @ &m: mem BR1.r Log.qs]
+    = Pr[CPA(BR2,A).main() @ &m: mem BR2.r Log.qs].
+  proof.
+    byequiv=> //=.
+    proc.
+    call (_:    ={Log.qs, RO.m}
+             /\ BR1.r{1} = BR2.r{2}).
+      proc. inline *. auto.
+    inline CPA(BR1,A).SO.enc CPA(BR2,A).SO.enc.
+    wp. rnd (fun x => m{2} ^ x).
+    rnd. simplify.
+    wp. rnd.
+    call (_: ={Log.qs, RO.m}).
+      proc. inline *. auto.
+    inline *. auto.
+    progress.
+      algebra.
+      smt.
+      smt.
+      algebra.
+  qed.
 
- call (_ : ={RO.m,Log.qs} /\ (forall x, mem x (dom RO.m){1} = mem x Log.qs{1})).
- proc;inline RO.o;wp;rnd;wp;skip;progress=> //.
-   by rewrite dom_set !mem_add H.
-   by rewrite mem_add; rewrite -H; case (x1 = x{2})=> //=;
-      intros=> ->; smt.
- wp;rnd;swap{1} -7;wp.
- call (_: ={RO.m,Log.qs}  /\ (forall x, mem x (dom RO.m){1} = mem x Log.qs{1})).
- proc;inline RO.o;wp;rnd;wp;skip;progress=> //.
-   by rewrite dom_set !mem_add H.
-   by rewrite mem_add; rewrite -H; case (x1 = x{2})=> //=;
-      intros=> ->; smt.
- do 2! (wp;rnd);skip;progress;smt.
- wp;skip;progress;first smt.
- pose eq_test:= fun p0 (p1:plaintext), p0 = x{2}.
- cut ->: (fun p0 (p1:plaintext), f pk{2} p0 = f pk{2} x{2}) = eq_test.
-   apply fun_ext=> y //=.
-   apply fun_ext=> y' //=.
-   rewrite eq_iff /eq_test; split=> //=.
-   by apply (f_iny _ _ _ sk{2} H).
- cut: exist eq_test RO.m{2}.
-   by rewrite /exist; exists x{2}=> //=; rewrite H0.
- cut find_cor: forall y, find eq_test RO.m{2} = Some y => x{2} = y.
-   by rewrite /eq_test; move=> y /find_cor.
- rewrite find_in /oget.
- by case {-1}(find eq_test RO.m{2}) (Logic.eq_refl (find eq_test RO.m{2})).
-qed.
+  (** Exercise: What single "equiv" lemma could be used to prove both
+      BR1_BR2 and BR1_BR2_bad in one? Prove it and use it to prove
+      BR1_BR2_bad and BR1_BR2. **)
 
-lemma Reduction &m : 
-Pr[CPA(BR,A).main() @ &m : res] <= 1%r / 2%r + Pr[OW(BR_OW(A)).main() @ &m : res].
-proof.
- apply (Real.Trans _  
-               (1%r/2%r + Pr[CPA2(BR2,A).main() @ &m : mem M.r Log.qs])).
- apply (prob1_2 &m) => //.
- cut H: (Pr[CPA2(BR2,A).main() @ &m : mem M.r Log.qs] <=
-         Pr[OW(BR_OW(A)).main() @ &m : res]).
-   byequiv eq2 => //.
- by smt.
-qed.
+  (** We can now prove that the success probability of A in CPA(BR2) is exactly 1/2 **)
+  local lemma pr_BR2_res &m: Pr[CPA(BR2,A).main() @ &m: res] = 1%r / 2%r.
+  proof.
+    byphoare=> //=.
+    proc.
+    inline CPA(BR2, A).SO.enc.
+    swap 6 4; swap 4 5.
+    wp.
+    rnd (pred1 b')=> //=.
+    inline *.
+    call (_: true). 
+      exact a2_ll. (* adversary *)
+      exact lossless_ARO_o. (* oracle *)
+    auto.
+    call (_: true).
+      exact a1_ll. (* adversary *)
+      exact lossless_ARO_o.
+    auto=> //=.
+    smt.
+  qed.
 
-lemma Conclusion  &m :
-exists (I<:Inverter), Pr[CPA(BR,A).main() @ &m : res] - 1%r / 2%r <= 
-                      Pr[OW(I).main() @ &m : res].
-proof.
- exists (BR_OW(A)). 
- by cut h := Reduction &m => //;smt.
-qed.
+  local lemma pr_BR_BR2 &m:
+    Pr[CPA(BR,A).main() @ &m: res] - 1%r/2%r
+    <= Pr[CPA(BR2,A).main() @ &m: mem BR2.r Log.qs].
+  proof. smt. qed.
 
+  (** Step 3: Finally, we can do the reduction and prove that whenever
+      A queries the RO with the randomness used in the challenge
+      encryption, BR_OW(A) inverts the OW challenge. **)
+  local lemma BR2_OW &m:
+    Pr[CPA(BR2,A).main() @ &m: mem BR2.r Log.qs]
+    <= Pr[OW(BR_OW(A)).main() @ &m: res].
+  proof.
+    byequiv => //=.
+    proc; inline *; wp.
+    (* simplify postcondition to no longer have find *)
+    conseq
+      (_ : _ ==>
+           support keypairs (pk0{2}, sk{2}) /\
+           BR2.r{1} = OW.r{2} /\ Log.qs{1} = Log.qs{2} /\
+           y{2} = f pk0{2} BR2.r{1}).
+      progress.
+      rewrite (find_unique OW.r{2} _ Log.qs{2}) => //=.
+      progress; first apply (f_injective sk{2} pk0{2} x OW.r{2}) => //.
+    (* rest of proof *)
+    swap {1} 3 - 2; swap {1} 9 -7; swap {1} 9 3; swap {1} 7 4.
+    wp. rnd{1}.
+    call (_: ={RO.m, Log.qs}); first by sim.
+    auto.
+    call (_: ={RO.m, Log.qs}); first by sim.
+    auto; smt.
+  qed.
+
+  lemma Reduction &m:
+    Pr[CPA(BR,A).main() @ &m : res] - 1%r/2%r
+    <= Pr[OW(BR_OW(A)).main() @ &m: res].
+  proof. smt. qed.
 end section.
